Core/Term.lean
@@ -1,3 +1,4 @@
 import Core.Term.Definition
 import Core.Term.BEq
 import Core.Term.Substitution
+import Core.Term.Utils
